src/PermDiskLog.v
@@ -92,14 +92,14 @@ Inductive state :=
 .
 
 Definition ent_addr (e : entry) := addr2w (fst e).
-Definition ent_block (e : entry) := fst (snd e).
+Definition ent_block (e : entry) := snd e.
 Definition ent_tag (e : entry) := fst (snd e).
 Definition ent_valu (e : entry) := snd (snd e).
 
 Definition ndesc_log (log : contents) := (divup (length log) DescSig.items_per_val).
 Definition ndesc_list T (l : list T) := (divup (length l) DescSig.items_per_val).
 
-Fixpoint log_nonzero (log : contents) : list entry :=
+Fixpoint log_nonzero (log : contents) : contents :=
   match log with
   | (0, _) :: rest => log_nonzero rest
   | e :: rest => e :: log_nonzero rest
@@ -168,7 +168,8 @@ Definition loglen_invalid xp ndesc ndata :=
   ndesc > LogDescLen xp \/ ndata > LogLen xp.
 
 Definition checksums_match (l : contents) h hm :=
-  hash_list_rep (rev (DescDefs.ipack (map ent_addr l))) (fst h) hm /\
+  hash_list_rep (rev (combine (addr_tags (ndesc_log l))
+                              (DescDefs.ipack (map ent_addr l)))) (fst h) hm /\
   hash_list_rep (rev (blocks_nonzero l)) (snd h) hm.
 
 Definition hide_or (P : Prop) := P.
@@ -178,7 +179,7 @@ Definition rep_inner xp (st : state) hm : rawpred :=
   (match st with
    | Synced l =>
      exists prev_len h,
-     Hdr.rep xp (Hdr.Synced (prev_len,
+     PermDiskLogHdr.rep xp (PermDiskLogHdr.Synced (prev_len,
                              (ndesc_log l, ndata_log l),
                              h)) *
      rep_contents xp l *
@@ -186,15 +187,15 @@ Definition rep_inner xp (st : state) hm : rawpred :=
        
    | Truncated old =>
      exists prev_len h h',
-     Hdr.rep xp (Hdr.Unsync ((ndesc_log old, ndata_log old), (0, 0), h')
+     PermDiskLogHdr.rep xp (PermDiskLogHdr.Unsync ((ndesc_log old, ndata_log old), (0, 0), h')
                             (prev_len, (ndesc_log old, ndata_log old), h)) *
      rep_contents xp old *
      [[ checksums_match old h hm ]] *
-     [[ checksums_match [] h' hm ]]
+     [[ checksums_match nil h' hm ]]
        
    | Extended old new =>
      exists prev_len h h',
-     Hdr.rep xp (Hdr.Unsync ((ndesc_log old, ndata_log old),
+     PermDiskLogHdr.rep xp (PermDiskLogHdr.Unsync ((ndesc_log old, ndata_log old),
                              (ndesc_log old + ndesc_log new,
                               ndata_log old + ndata_log new), h')
                             (prev_len, (ndesc_log old, ndata_log old), h)) *
@@ -206,12 +207,12 @@ Definition rep_inner xp (st : state) hm : rawpred :=
      [[ Forall entry_valid new ]]
        
    | ExtendedCrashed old new =>
-     exists h synced_addr synced_valu ndesc,
-     Hdr.rep xp (Hdr.Synced ((ndesc_log old, ndata_log old),
+     exists h synced_addr synced_tag synced_valu ndesc,
+     PermDiskLogHdr.rep xp (PermDiskLogHdr.Synced ((ndesc_log old, ndata_log old),
                              (ndesc_log old + ndesc_log new,
                               ndata_log old + ndata_log new),
                              h)) *
-     rep_contents_unmatched xp old synced_addr synced_valu *
+     rep_contents_unmatched xp old synced_addr synced_tag synced_valu *
      [[ loglen_valid xp (ndesc_log old + ndesc_log new)
                      (ndata_log old + ndata_log new) ]] *
      (* Whatever got synced on disk takes up just as many desc blocks as new should've. *)
@@ -222,12 +223,12 @@ Definition rep_inner xp (st : state) hm : rawpred :=
      [[ Forall entry_valid new ]]
        
    | Rollback old =>
-     exists synced_addr synced_valu h new,
-     Hdr.rep xp (Hdr.Synced ((ndesc_log old, ndata_log old),
+     exists synced_addr synced_tag synced_valu h new,
+     PermDiskLogHdr.rep xp (PermDiskLogHdr.Synced ((ndesc_log old, ndata_log old),
                              (ndesc_log old + ndesc_log new,
                               ndata_log old + ndata_log new),
                              h)) *
-     rep_contents_unmatched xp old synced_addr synced_valu *
+     rep_contents_unmatched xp old synced_addr synced_tag synced_valu *
      [[ loglen_valid xp (ndesc_log old + ndesc_log new)
                      (ndata_log old + ndata_log new) ]] *
      (* Whatever got synced on disk takes up just as many desc blocks as new should've. *)
@@ -239,12 +240,12 @@ Definition rep_inner xp (st : state) hm : rawpred :=
      [[ Forall entry_valid new ]]
        
   | RollbackUnsync old =>
-    exists synced_addr synced_valu h h' new prev_len,
-    Hdr.rep xp (Hdr.Unsync (prev_len, (ndesc_log old, ndata_log old), h')
+    exists synced_addr synced_tag synced_valu h h' new prev_len,
+    PermDiskLogHdr.rep xp (PermDiskLogHdr.Unsync (prev_len, (ndesc_log old, ndata_log old), h')
                            ((ndesc_log old, ndata_log old),
                             (ndesc_log old + ndesc_log new,
                              ndata_log old + ndata_log new), h)) *
-    rep_contents_unmatched xp old synced_addr synced_valu *
+    rep_contents_unmatched xp old synced_addr synced_tag synced_valu *
     [[ loglen_valid xp (ndesc_log old + ndesc_log new)
                     (ndata_log old + ndata_log new) ]] *
     (* Whatever got synced on disk takes up just as many desc blocks as new should've. *)
@@ -271,8 +272,8 @@ Definition would_recover' xp l hm :=
    rep xp (RollbackUnsync l) hm)%pred.
 
 Definition would_recover xp F l hm :=
-  (exists cs d,
-     BUFCACHE.rep cs d *
+  (exists cs d bm,
+     PermCacheDef.rep cs d bm *
      [[ (F * would_recover' xp l hm)%pred d ]])%pred.
 
 
@@ -301,5 +302,407 @@ Proof.
 Qed.
 
 Hint Resolve sync_invariant_would_recover sync_invariant_would_recover'.
-
 Local Hint Unfold rep rep_inner rep_contents xparams_ok: hoare_unfold.
+
+
+
+
+Definition unseal_all (hl: list handle) :=
+  let^ (bl) <- ForN i < length hl
+        Blockmem bm
+        Ghost [ crash ]
+        Loopvar [ tbl ]
+        Invariant
+           [[ rev (tbl) = map snd (extract_blocks bm (firstn i hl)) ]]
+        OnCrash
+           crash
+        Begin
+           tb <- Unseal (selN hl i 0);;
+           Ret ^(tb::tbl)
+       Rof ^((nil: list block));;
+  Ret (rev bl).
+
+Definition avail xp cs :=
+  let^ (cs, nr) <- PermDiskLogHdr.read xp cs;;
+    let '(_, (ndesc, _), _) := nr in
+    Ret ^(cs, ((LogLen xp) - ndesc * DescSig.items_per_val)).
+
+  Definition read xp cs :=
+    let^ (cs, nr) <- PermDiskLogHdr.read xp cs;;
+    let '(_, (ndesc, ndata), _) := nr in
+    let^ (cs, ahl) <- Desc.read_all xp ndesc cs;;
+    abl <- unseal_all ahl;;
+                   
+    let al := map (@wordToNat addrlen) wal in
+    let^ (cs, vl) <- Data.read_all xp ndata cs;;
+    Ret ^(cs, combine_nonzero al vl).
+
+  (* this is an evil hint *)
+  Remove Hints Forall_nil.
+
+  Lemma Forall_True : forall A (l : list A),
+    Forall (fun _ : A => True) l.
+  Proof.
+    intros; rewrite Forall_forall; auto.
+  Qed.
+  Hint Resolve Forall_True.
+
+  Lemma combine_nonzero_ok : forall l,
+    combine_nonzero (map fst l) (vals_nonzero l) = log_nonzero l.
+  Proof.
+    unfold vals_nonzero.
+    induction l; intros; simpl; auto.
+    destruct a, n; simpl.
+    case_eq (map ent_valu (log_nonzero l)); intros; simpl.
+    apply map_eq_nil in H; auto.
+    rewrite <- H; auto.
+    rewrite IHl; auto.
+  Qed.
+
+  Lemma combine_nonzero_nil : forall a,
+    combine_nonzero a nil = nil.
+  Proof.
+    induction a; intros; simpl; auto.
+    destruct a; simpl; auto.
+  Qed.
+  Local Hint Resolve combine_nonzero_nil.
+
+  Lemma combine_nonzero_app_zero : forall a b,
+    combine_nonzero (a ++ [0]) b = combine_nonzero a b.
+  Proof.
+    induction a; intros; simpl; auto.
+    destruct b; auto.
+    destruct a, b; simpl; auto.
+    rewrite IHa; auto.
+  Qed.
+
+  Lemma combine_nonzero_app_zeros : forall n a b,
+    combine_nonzero (a ++ repeat 0 n) b = combine_nonzero a b.
+  Proof.
+    induction n; intros; simpl.
+    rewrite app_nil_r; auto.
+    rewrite <- cons_nil_app.
+    rewrite IHn.
+    apply combine_nonzero_app_zero.
+  Qed.
+
+  Local Hint Resolve roundup_ge DescDefs.items_per_val_gt_0.
+
+  Lemma combine_nonzero_padded_addr : forall a b,
+    combine_nonzero (padded_addr a) b = combine_nonzero a b.
+  Proof.
+    unfold padded_addr, vals_nonzero.
+    induction a; intros; simpl; auto.
+    unfold setlen, roundup; simpl.
+    rewrite divup_0; simpl; auto.
+
+    unfold setlen, roundup; simpl.
+    destruct a, b; simpl; auto;
+    rewrite firstn_oob; simpl; auto;
+    rewrite combine_nonzero_app_zeros; auto.
+  Qed.
+
+  Lemma map_fst_repeat : forall A B n (a : A) (b : B),
+    map fst (repeat (a, b) n) = repeat a n.
+  Proof.
+    induction n; intros; simpl; auto.
+    rewrite IHn; auto.
+  Qed.
+
+  Lemma map_entaddr_repeat_0 : forall n b,
+    map ent_addr (repeat (0, b) n) = repeat $0 n.
+  Proof.
+    induction n; intros; simpl; auto.
+    rewrite IHn; auto.
+  Qed.
+
+  Lemma combine_nonzero_padded_log : forall l b,
+    combine_nonzero (map fst (padded_log l)) b = combine_nonzero (map fst l) b.
+  Proof.
+    unfold padded_log, setlen, roundup; intros.
+    induction l; simpl.
+    rewrite divup_0; simpl; auto.
+    
+    rewrite <- IHl.
+    destruct a, b, n; simpl; auto;
+    repeat rewrite firstn_oob; simpl; auto;
+    repeat rewrite map_app;
+    setoid_rewrite map_fst_repeat;
+    repeat rewrite combine_nonzero_app_zeros; auto.
+  Qed.
+
+  Lemma addr_valid_padded : forall l,
+    Forall addr_valid l -> Forall addr_valid (padded_log l).
+  Proof.
+    unfold padded_log, setlen, roundup; intros.
+    rewrite firstn_oob; simpl; auto.
+    apply Forall_append; auto.
+    rewrite Forall_forall; intros.
+    apply repeat_spec in H0; subst.
+    unfold addr_valid; simpl.
+    apply zero_lt_pow2.
+  Qed.
+
+  Lemma padded_addr_valid : forall l,
+    Forall addr_valid (padded_log l) ->
+    Forall addr_valid l.
+  Proof.
+    unfold padded_log, setlen; intros.
+    rewrite firstn_oob in H; auto.
+    eapply forall_app_r; eauto.
+  Qed.
+
+  Local Hint Resolve addr_valid_padded padded_addr_valid.
+
+  Lemma map_wordToNat_ent_addr : forall l,
+    Forall addr_valid l ->
+    (map (@wordToNat _) (map ent_addr l)) = map fst l.
+  Proof.
+    unfold ent_addr, addr2w.
+    induction l; intros; simpl; auto.
+    rewrite IHl; f_equal.
+    rewrite wordToNat_natToWord_idempotent'; auto.
+    apply Forall_inv in H; unfold addr_valid in H; auto.
+    eapply Forall_cons2; eauto.
+  Qed.
+
+  Lemma combine_nonzero_padded_wordToNat : forall l,
+    Forall addr_valid l ->
+    combine_nonzero (map (@wordToNat _) (map ent_addr (padded_log l))) (vals_nonzero l) = log_nonzero l.
+  Proof.
+    intros; unfold ent_addr, addr2w.
+    rewrite <- combine_nonzero_ok.
+    rewrite <- combine_nonzero_padded_log.
+    f_equal.
+    rewrite map_wordToNat_ent_addr; auto.
+  Qed.
+
+  Lemma vals_nonzero_addrs : forall l,
+    length (vals_nonzero l) = nonzero_addrs (map fst l).
+  Proof.
+    induction l; intros; simpl; auto.
+    destruct a, n; simpl; auto.
+  Qed.
+
+  Lemma log_nonzero_addrs : forall l,
+    length (log_nonzero l) = nonzero_addrs (map fst l).
+  Proof.
+    induction l; intros; simpl; auto.
+    destruct a, n; simpl; auto.
+  Qed.
+
+  Lemma desc_ipack_padded : forall l,
+    DescDefs.ipack (map ent_addr l) = DescDefs.ipack (map ent_addr (padded_log l)).
+  Proof.
+    unfold padded_log, setlen; intros.
+    rewrite firstn_oob, map_app, map_entaddr_repeat_0 by auto.
+    rewrite DescDefs.ipack_app_item0; auto.
+    rewrite map_length; auto.
+  Qed.
+
+  Local Hint Resolve combine_nonzero_padded_wordToNat.
+
+  Lemma desc_padding_synced_piff : forall xp a l,
+    Desc.array_rep xp a (Desc.Synced (map ent_addr (padded_log l)))
+    <=p=> Desc.array_rep xp a (Desc.Synced (map ent_addr l)).
+  Proof.
+     unfold Desc.array_rep, Desc.synced_array, Desc.rep_common; intros.
+     split; cancel; subst.
+     unfold padded_log, setlen, roundup in H0.
+     rewrite firstn_oob, map_app in H0 by auto.
+     apply Desc.items_valid_app in H0; intuition.
+     apply eq_sym; apply desc_ipack_padded.
+     unfold padded_log, setlen, roundup.
+     rewrite firstn_oob, map_app by auto.
+     apply Desc.items_valid_app2; auto.
+     autorewrite with lists; auto.
+     apply desc_ipack_padded.
+  Qed.
+
+  Lemma desc_padding_unsync_piff : forall xp a l,
+    Desc.array_rep xp a (Desc.Unsync (map ent_addr (padded_log l)))
+    <=p=> Desc.array_rep xp a (Desc.Unsync (map ent_addr l)).
+  Proof.
+     unfold Desc.array_rep, Desc.unsync_array, Desc.rep_common; intros.
+     split; cancel; subst.
+     unfold padded_log, setlen, roundup in H.
+     rewrite firstn_oob, map_app in H by auto.
+     apply Desc.items_valid_app in H; intuition.
+     apply eq_sym; apply desc_ipack_padded.
+     unfold padded_log, setlen, roundup.
+     rewrite firstn_oob, map_app by auto.
+     apply Desc.items_valid_app2; auto.
+     autorewrite with lists; auto.
+     apply desc_ipack_padded.
+  Qed.
+
+  Lemma goodSize_ndesc : forall l,
+    goodSize addrlen (length l) -> goodSize addrlen (ndesc_log l).
+  Proof.
+    intros; unfold ndesc_log.
+    eapply goodSize_trans; [ apply divup_le | eauto ].
+    destruct (mult_O_le (length l) DescSig.items_per_val); auto.
+    contradict H0; apply DescDefs.items_per_val_not_0.
+  Qed.
+  Local Hint Resolve goodSize_ndesc.
+
+  Lemma padded_log_length: forall l,
+    length (padded_log l) = roundup (length l) DescSig.items_per_val.
+  Proof.
+    unfold padded_log, roundup; intros.
+    rewrite setlen_length; auto.
+  Qed.
+
+  Lemma nonzero_addrs_app_zero : forall a,
+    nonzero_addrs (a ++ [0]) = nonzero_addrs a.
+  Proof.
+    induction a; intros; simpl; auto.
+    destruct a; simpl; auto.
+  Qed.
+
+  Lemma nonzero_addrs_app_zeros : forall n a,
+    nonzero_addrs (a ++ repeat 0 n) = nonzero_addrs a.
+  Proof.
+    induction n; intros; simpl.
+    rewrite app_nil_r; auto.
+    rewrite <- cons_nil_app.
+    rewrite IHn.
+    apply nonzero_addrs_app_zero.
+  Qed.
+
+  Lemma nonzero_addrs_padded_log : forall l,
+    nonzero_addrs (map fst (padded_log l)) = nonzero_addrs (map fst l).
+  Proof.
+    unfold padded_log; induction l; simpl; auto.
+    rewrite setlen_nil, repeat_is_nil; simpl; auto.
+    unfold roundup; rewrite divup_0; omega.
+    
+    destruct a, n; simpl;
+    rewrite <- IHl;
+    unfold setlen, roundup;
+    repeat rewrite firstn_oob, map_app by auto;
+    setoid_rewrite map_fst_repeat;
+    repeat rewrite nonzero_addrs_app_zeros; simpl; auto.
+  Qed.
+
+  Lemma vals_nonzero_length : forall l,
+    length (vals_nonzero l) <= length l.
+  Proof.
+    unfold vals_nonzero; induction l; intros; simpl; auto.
+    destruct a, n; simpl; auto.
+    autorewrite with lists in *; omega.
+  Qed.
+
+  Lemma vals_nonzero_app : forall a b,
+    vals_nonzero (a ++ b) = vals_nonzero a ++ vals_nonzero b.
+  Proof.
+    unfold vals_nonzero; induction a; intros; simpl; auto.
+    destruct a, n; simpl; auto.
+    rewrite IHa; auto.
+  Qed.
+
+  Lemma log_nonzero_repeat_0 : forall n,
+    log_nonzero (repeat (0, $0) n) = nil.
+  Proof.
+    induction n; simpl; auto.
+  Qed.
+
+  Lemma log_nonzero_app : forall a b,
+    log_nonzero (a ++ b) = log_nonzero a ++ log_nonzero b.
+  Proof.
+    induction a; simpl; intros; auto.
+    destruct a, n; simpl; auto.
+    rewrite IHa; auto.
+  Qed.
+
+  Lemma vals_nonzero_padded_log : forall l,
+    vals_nonzero (padded_log l) = vals_nonzero l.
+  Proof.
+    unfold vals_nonzero, padded_log, setlen, roundup; simpl.
+    induction l; intros; simpl; auto.
+    rewrite firstn_oob; simpl; auto.
+    rewrite log_nonzero_repeat_0; auto.
+
+    destruct a, n.
+    rewrite <- IHl.
+    repeat rewrite firstn_oob; simpl; auto.
+    repeat rewrite log_nonzero_app, map_app.
+    repeat rewrite log_nonzero_repeat_0; auto.
+
+    repeat rewrite firstn_oob; simpl; auto.
+    f_equal.
+    repeat rewrite log_nonzero_app, map_app.
+    repeat rewrite log_nonzero_repeat_0; auto.
+    simpl; rewrite app_nil_r; auto.
+  Qed.
+
+  Lemma ndata_log_goodSize : forall l,
+    goodSize addrlen (length l) -> goodSize addrlen (ndata_log l).
+  Proof.
+    unfold ndata_log; intros.
+    rewrite <- vals_nonzero_addrs.
+    eapply goodSize_trans.
+    apply vals_nonzero_length; auto.
+    auto.
+  Qed.
+  Local Hint Resolve ndata_log_goodSize.
+
+  Lemma padded_log_idem : forall l,
+    padded_log (padded_log l) = padded_log l.
+  Proof.
+    intros.
+    unfold padded_log.
+    rewrite setlen_length.
+    rewrite roundup_roundup; auto.
+    rewrite setlen_exact; auto.
+    rewrite setlen_length; auto.
+  Qed.
+
+  Lemma padded_log_app : forall l1 l2,
+    padded_log (padded_log l1 ++ l2) = padded_log l1 ++ padded_log l2.
+  Proof.
+    intros.
+    unfold padded_log.
+    rewrite setlen_app_r.
+    f_equal.
+    rewrite app_length, setlen_length.
+    rewrite roundup_roundup_add; auto.
+    f_equal; omega.
+    rewrite app_length, setlen_length.
+    rewrite roundup_roundup_add; auto.
+    omega.
+  Qed.
+
+  Ltac solve_checksums :=
+  try (match goal with
+    | [ |- checksums_match _ _ _ ]
+      => unfold checksums_match in *
+    end; intuition;
+    [
+      solve_hash_list_rep;
+      try (rewrite map_app;
+      erewrite DescDefs.ipack_app;
+      try solve [ rewrite map_length, padded_log_length; unfold roundup; eauto ];
+      rewrite rev_app_distr)
+      | solve_hash_list_rep;
+      try rewrite vals_nonzero_app, vals_nonzero_padded_log, rev_app_distr;
+      try rewrite padded_log_app, map_app, rev_app_distr
+    ];
+    repeat match goal with
+    | [ H: context[hash_list_rep (_ ++ [])] |- _ ]
+      => rewrite app_nil_r in H
+    end;
+    try rewrite <- desc_ipack_padded in *;
+    solve_hash_list_rep).
+
+
+  Arguments Desc.array_rep : simpl never.
+  Arguments Data.array_rep : simpl never.
+  Arguments Desc.avail_rep : simpl never.
+  Arguments Data.avail_rep : simpl never.
+  Arguments divup : simpl never.
+  Hint Extern 0 (okToUnify (Hdr.rep _ _) (Hdr.rep _ _)) => constructor : okToUnify.
+  Hint Extern 0 (okToUnify (Desc.array_rep _ _ _) (Desc.array_rep _ _ _)) => constructor : okToUnify.
+  Hint Extern 0 (okToUnify (Data.array_rep _ _ _) (Data.array_rep _ _ _)) => constructor : okToUnify.
+  Hint Extern 0 (okToUnify (Desc.avail_rep _ _ _) (Desc.avail_rep _ _ _)) => constructor : okToUnify.
+  Hint Extern 0 (okToUnify (Data.avail_rep _ _ _) (Data.avail_rep _ _ _)) => constructor : okToUnify.
