src/PermCacheRangeSec.v
@@ -1,0 +1,211 @@
+Require Import List.
+Require Import FMapAVL.
+Require Import FMapFacts.
+Require Import Word.
+Require Import PermArray.
+Require Import Pred.
+Require Import WordAuto.
+Require Import Omega.
+Require Import ListUtils.
+Require Import OrderedTypeEx.
+Require Import Arith.
+Require Import MapUtils.
+Require Import MemPred.
+Require Import ListPred. 
+Require Import FunctionalExtensionality.
+Require Import ADestructPair DestructVarname.
+Require Export PermCacheSec.
+
+
+Import AddrMap.
+Import Map MapFacts.
+Import ListNotations.
+
+Set Implicit Arguments.
+
+
+  Theorem read_range_ok :
+    forall a nr cs pr,
+    {< d F vs,
+    PERM: pr   
+    PRE:bm, hm,
+        rep cs d bm *
+        [[ (F * arrayS a vs)%pred d ]] *
+        [[ nr <= length vs ]]
+   POST:bm', hm',
+      RET:^(cs, r)
+       rep cs d bm' *
+      [[ extract_blocks bm' r = firstn nr (List.map fst vs)]]
+    CRASH:bm'', hm'',
+      exists cs', rep cs' d bm''
+    >} read_range a nr cs.
+  Proof.
+    unfold read_range; intros.
+    step.
+    step.
+
+    step.
+    step.
+
+    erewrite firstn_S_selN_expand.
+    erewrite selN_map; auto.
+    rewrite extract_blocks_app; simpl.
+    rewrite H17.
+    destruct (find (a + length a1) (CSMap a0)); try logic_clean; subst.
+    rewrite H13; auto.
+
+    destruct (in_dec handle_eq_dec a3 a1).
+    pose proof (extract_blocks_length_lt _ _ _ i e0).
+    assert (A: length(extract_blocks bm0 (rev a1)) =
+               length (firstn (length a1) (List.map fst vs))).
+    rewrite H13; auto.
+    rewrite firstn_length_l in A.
+    rewrite extract_blocks_rev_length_eq, A in H9; omega.
+    rewrite map_length.
+    eapply le_trans; [| eauto].
+    omega.
+
+    rewrite extract_blocks_upd_not_in; eauto.
+    rewrite H13; auto.
+    Search List.In rev.
+    unfold not; intros Hx;
+    apply in_rev in Hx; auto.
+    eapply le_trans; [| eauto]; omega.
+    rewrite map_length.
+    eapply le_trans; [| eauto].
+    omega.
+
+    eexists; repeat (eapply hashmap_subset_trans; eauto).
+    rewrite <- H1; cancel; eauto.
+    eexists; repeat (eapply hashmap_subset_trans; eauto).
+
+    step.
+    step.
+    eexists; repeat (eapply hashmap_subset_trans; eauto).
+    rewrite <- H1; cancel.
+    eauto.
+    eexists; repeat (eapply hashmap_subset_trans; eauto).
+
+    Unshelve. all: eauto.
+    exact tt.
+    unfold EqDec; apply handle_eq_dec.
+    exact tagged_block0.
+    unfold EqDec; apply handle_eq_dec.
+  Qed.
+
+
+  Theorem write_range_ok :
+    forall a l cs pr,
+    {< d F vs vsl,
+    PERM: pr   
+    PRE:bm, hm,
+      rep cs d bm *
+      [[ (F * arrayS a vs)%pred d ]] *
+      [[ length l <= length vs ]] *
+      [[ vsl = extract_blocks bm l ]] *
+      [[ length l = length vsl ]]
+    POST:bm', hm', RET:cs
+      exists d', rep cs d' bm' *
+      [[ (F * arrayS a (vsupd_range vs vsl))%pred d' ]]
+    XCRASH:bm'', hm'',
+      exists cs' d', rep cs' d' bm''*
+      [[ (F * arrayS a (vsupd_range vs vsl))%pred d' ]]
+    >} write_range a l cs.
+  Proof.
+    unfold write_range; intros.
+    step.
+    prestep; unfold rep; cancel.
+    subst.
+
+    erewrite extract_blocks_selN.
+    rewrite <- H15; eauto.
+    rewrite <- H15; auto.
+    auto.
+    
+    rewrite vsupd_range_length; try omega.
+    eapply lt_le_trans; eauto.
+    rewrite firstn_length_l; try omega.
+    eapply le_trans; [|eauto].
+    apply Nat.lt_le_incl; auto.
+    rewrite <- H5; apply Nat.lt_le_incl; auto.
+
+    step.
+    prestep; unfold rep; cancel.
+    erewrite firstn_S_selN_expand.
+    setoid_rewrite <- vsupd_range_progress; auto.
+
+    cancel.
+    all: try rewrite <- H5; auto.
+    eexists; repeat (eapply hashmap_subset_trans; eauto).
+    
+    rewrite <- H1; cancel; eauto.
+    eexists; repeat (eapply hashmap_subset_trans; eauto).
+    repeat xcrash_rewrite.
+    setoid_rewrite vsupd_range_progress; auto.
+    rewrite <- firstn_plusone_selN.
+
+    apply vsupd_range_xcrash_firstn; auto.
+    all: try rewrite <- H5; auto.
+
+    step. step.
+    rewrite firstn_oob; auto.
+    rewrite <- H5; auto.
+    eexists; repeat (eapply hashmap_subset_trans; eauto).
+    eassign (false_pred (AT:= addr)(AEQ:= addr_eq_dec)(V:= valuset))%pred.
+    rewrite <- H1; cancel; eauto.
+    unfold false_pred, crash_xform.
+    unfold pimpl; intros; simpl in *; cleanup; intuition.
+    Unshelve.
+    exact tt.
+    unfold EqDec; apply handle_eq_dec.
+  Qed.
+
+
+  Theorem sync_range_ok :
+    forall a n cs pr,
+    {< d d0 F vs,
+    PERM: pr   
+    PRE:bm, hm,
+      synrep cs d0 d bm *
+      [[ (F * arrayS a vs)%pred d ]] *
+      [[ n <= length vs /\ sync_invariant F ]]
+    POST:bm', hm', RET:cs
+      exists d', synrep cs d0 d' bm' *
+      [[ (F * arrayS a (vssync_range vs n))%pred d' ]]
+    CRASH:bm'', hm'',
+      exists cs', rep cs' d0 bm''
+    >} sync_range a n cs.
+  Proof.
+    unfold sync_range; intros.
+    safestep.
+    eassign F_; cancel.
+    unfold vssync_range; simpl; eauto.
+    eauto.
+    eauto.
+    safestep.
+    eassign F_; cancel.
+    eauto.
+    rewrite vssync_range_length; omega.
+    all: auto.
+
+    step. step.
+    apply arrayN_unify.
+    apply vssync_range_progress; omega.
+    eexists; repeat (eapply hashmap_subset_trans; eauto).
+    rewrite <- H1; cancel; eauto.
+    eexists; repeat (eapply hashmap_subset_trans; eauto).
+    
+    step.step.
+    eexists; repeat (eapply hashmap_subset_trans; eauto).
+    rewrite <- H1; cancel; eauto.
+    
+    Unshelve.
+    exact tt.
+    unfold EqDec; apply handle_eq_dec.
+    auto.
+  Qed.
+
+
+  Hint Extern 1 ({{_|_}} Bind (read_range _ _ _) _) => apply read_range_ok : prog.
+  Hint Extern 1 ({{_|_}} Bind (write_range _ _ _) _) => apply write_range_ok : prog.
+  Hint Extern 1 ({{_|_}} Bind (sync_range _ _ _) _) => apply sync_range_ok : prog.
